Q4

ex2/imp.v
@@ -1,7 +1,11 @@
 Set Implicit Arguments.
+Require Import Coq.Program.Equality.
+Require Import Lia.
 
 
 Inductive var := a | b | n | x | y.
+
+Scheme Equality for var.
 
 Definition op := nat -> nat -> nat.
   
@@ -28,7 +32,7 @@ Fixpoint sem (e : expr) (s : state) :=
   end.
 
 
-(* -- Defining the program `euclid` in IMP -- *)
+(* -- Defining the program euclid in IMP -- *)
 Require Import Arith.
 Import Nat.
 
@@ -44,3 +48,86 @@ Definition euclid_body :=
         (if_then_else (expr_op $a gt01 $b)
                       (assign a (expr_op $a sub $b))
                       (assign b (expr_op $b sub $a))).
+
+
+(* ----------------------- *)
+
+Inductive sos   : (state * cmd) -> (state * cmd) -> Prop :=
+(* assign *)
+  | sos_assign : forall s v e,
+      sos (s, assign v e) ((fun x => if var_eq_dec x v then sem e s else s x), skip)
+(* seq *)
+  | sos_seq : forall s s' c1 c1' c2,
+      sos (s, c1) (s', c1') -> sos (s, seq c1 c2) (s', seq c1' c2)
+  | sos_seq_skip : forall s c2,
+      sos (s, seq skip c2) (s, c2)
+(* if_then_else *)
+  | sos_if_true  : forall s e c1 c2,
+      sem e s <> 0 -> sos (s, if_then_else e c1 c2) (s, c1)
+  | sos_if_false : forall s e c1 c2,
+      sem e s = 0 -> sos (s, if_then_else e c1 c2) (s, c2)
+(* while *)
+  | sos_while_true : forall s e c,
+      sem e s <> 0 -> sos (s, while e c) (s, seq c (while e c))
+  | sos_while_false : forall s e c,
+      sem e s = 0 -> sos (s, while e c) (s, skip)      
+(* assume *)
+  | sos_assume_true : forall s e,
+      sem e s <> 0 -> sos (s, assume e) (s, skip).
+
+
+Inductive step : state -> state -> Prop :=
+  | step_a : forall s,
+      s a > s b ->
+      step s (fun x => if var_eq_dec x a then s a - s b else s x)
+  | step_b : forall s,
+      s a < s b ->
+      step s (fun x => if var_eq_dec x b then s b - s a else s x).
+
+  (* tc definitions from lab 5, changed to match step and sos *) 
+  Inductive tc' (R: state -> state -> Prop): state -> state -> Prop :=
+    tc'_refl : forall s, (tc' R) s s
+  | tc'_step : forall s u t, R s u -> (tc' R) u t -> (tc' R) s t.
+
+(* our implementation of gcd (eucalid version *)  
+Inductive euclid : nat -> nat -> nat -> Prop :=
+  stop    : forall z, euclid z z z
+| step_a' : forall a b z, a > b -> euclid (a - b) b z -> euclid a b z
+| step_b' : forall a b z, a < b -> euclid a (b - a) z -> euclid a b z. 
+
+Lemma step_correctness : forall a0 b0 s s' , 
+                             s a = a0 -> 
+                             s b = b0 -> 
+                             (tc' step) s s' -> 
+                             s' a = s' b ->
+                                 euclid a0 b0 (s' a).
+Proof.
+intros a0 b0 s s' Ha Hb Htc.
+  generalize dependent a0.
+  generalize dependent b0.
+  induction Htc as [| s u t Hstep Htc' IH]; intros b0 a0 Ha Hb Heq.
+  - (* base case a = b = z *)
+    subst. rewrite Heq. apply stop.
+
+  - (* inductive step *)
+    destruct Hstep.
+
+    + (* case a > b, so a := a - b *)
+      apply step_a'. subst.
+      assumption.
+      apply IH.
+      * (* a0' := s a - s b *)
+        simpl. subst. reflexivity.
+      * (* b0' := s b *)
+        simpl. subst. reflexivity.
+      * assumption.
+      
+    + (* case a < b, so b := b - a *)
+      apply step_b'. subst. assumption.
+      apply IH.
+      * (* a0 := s a *)
+        simpl. subst. lia.
+      * (* b0 := s b - s a *)
+        simpl. assumption.
+      * assumption. 
+Qed.
